Split dot_lty for reuse

theories/misc_unused/lty_experiments.v
@@ -88,180 +88,21 @@ End judgments.
 
 End Lty_judge.
 
-From D.Dot Require Import syn lr_syn_aux dlang_inst rules typeExtractionSyn path_wp typeExtractionSem.
-From D.Dot.syn Require Import path_repl.
-From D.Dot Require unary_lr.
-From D.Dot.lr Require path_repl.
+From D.Dot Require Import syn lr_syn_aux syn.path_repl typeExtractionSyn.
+From D.Dot Require Import dlang_inst path_wp dot_lty.
+
+From D.Dot.lr Require unary_lr path_repl.
 
 Implicit Types
          (v: vl) (e: tm) (d: dm) (ds: dms) (p : path).
 
-Module SemTypes.
+Module SemTypes2.
 
-Include LtyJudgements VlSorts dlang_inst.
+Import SemTypes.
 
-Record dlty Σ := Dlty {
-  dlty_label : label;
-  dlty_car : env -d> dm -d> iPropO Σ;
-  dlty_persistent ρ d :> Persistent (dlty_car ρ d);
-}.
-Global Arguments Dlty {_} _%I _ {_}.
-Global Arguments dlty_car {_} !_ _ _ /.
-Global Arguments dlty_label {_} _ /.
-Global Existing Instance dlty_persistent.
-
-Definition sdtp `{!dlangG Σ} Γ l (φ : dlty Σ) d : iProp Σ :=
-  (⌜ l = dlty_label φ ⌝ ∧
-    □∀ ρ, s⟦Γ⟧* ρ → dlty_car φ ρ d.|[ρ])%I.
-Global Arguments sdtp /.
-Notation "Γ s⊨ { l := d  } : T" := (sdtp Γ l T d) (at level 64, d, l, T at next level).
-
-Definition sptp `{!dlangG Σ} Γ (τ : olty Σ 0) p i: iProp Σ :=
-  □∀ ρ, s⟦Γ⟧* ρ -∗
-    ▷^i path_wp (p.|[ρ]) (λ v, oClose τ ρ v).
-
-Notation "Γ s⊨p p : τ , i" := (sptp Γ τ p i) (at level 74, p, τ, i at next level).
-
-Section SemTypes.
+Section with_unary_lr.
   Context `{HdotG: dlangG Σ}.
 
-  Implicit Types (τ : olty Σ 0).
-   (* (ψ : vl -d> iPropO Σ) (φ : envD Σ)  *)
-
-  Program Definition lift_dinterp_vl (T : dlty Σ): olty Σ 0 :=
-    olty0 (λ ρ v, (∃ d, ⌜v @ dlty_label T ↘ d⌝ ∧ dlty_car T ρ d)%I).
-
-  Definition dm_to_type d i (ψ : hoD Σ i) : iProp Σ :=
-    (∃ s σ, ⌜ d = dtysem σ s ⌝ ∧ s ↗n[ σ , i ] ψ)%I.
-  Notation "d ↗n[ i  ] ψ" := (dm_to_type d i ψ) (at level 20).
-  Global Instance dm_to_type_persistent d i ψ: Persistent (d ↗n[ i ] ψ) := _.
-
-  Lemma dm_to_type_agree d i ψ1 ψ2 args v : d ↗n[ i ] ψ1 -∗ d ↗n[ i ] ψ2 -∗ ▷ (ψ1 args v ≡ ψ2 args v).
-  Proof.
-    iDestruct 1 as (s σ ?) "#Hs1".
-    iDestruct 1 as (s' σ' ?) "#Hs2".
-    simplify_eq. by iApply (stamp_σ_to_type_agree args with "Hs1 Hs2").
-  Qed.
-
-  Lemma dm_to_type_intro d i s σ φ :
-    d = dtysem σ s → s ↝n[ i ] φ -∗ d ↗n[ i ] hoEnvD_inst σ φ.
-  Proof.
-    iIntros. iExists s, σ. iFrame "%".
-    by iApply stamp_σ_to_type_intro.
-  Qed.
-
-  Global Opaque dm_to_type.
-
-  (* Rewrite using (higher) semantic kinds! *)
-  Definition oDTMem l τ1 τ2 : dlty Σ := Dlty l
-    (λ ρ d,
-    ∃ ψ, (d ↗n[ 0 ] ψ) ∧
-       □ ((∀ v, ▷ τ1 vnil ρ v → ▷ □ ψ vnil v) ∧
-          (∀ v, ▷ □ ψ vnil v → ▷ τ2 vnil ρ v)))%I.
-
-  Definition oTTMem l τ1 τ2 :=
-    lift_dinterp_vl (oDTMem l τ1 τ2).
-
-  Definition oDVMem l τ : dlty Σ := Dlty l
-    (λ ρ d, ∃ pmem, ⌜d = dpt pmem⌝ ∧ path_wp pmem (oClose τ ρ))%I.
-
-  Definition oTVMem l τ :=
-    lift_dinterp_vl (oDVMem l τ).
-(*
-  Program Definition oInterp T := Olty ⟦ T ⟧ _.
-  Next Obligation. rewrite /vclosed=>*. by rewrite interp_vclosed. Qed. *)
-
-  Definition oTSel p (l : label) :=
-    olty0 (λ ρ v, path_wp p.|[ρ]
-      (λ vp, ∃ ψ d, ⌜vp @ l ↘ d⌝ ∧ d ↗n[ 0 ] ψ ∧ ▷ □ ψ vnil v))%I.
-
-  Lemma oTSel_pv w (l : label) args ρ v :
-    oTSel (pv w) l args ρ v ≡
-      (∃ ψ d, ⌜w.[ρ] @ l ↘ d⌝ ∧ d ↗n[ 0 ] ψ ∧ ▷ □ ψ vnil v)%I.
-  Proof. by rewrite /= path_wp_pv. Qed.
-
-  Lemma Sub_Sel Γ L U va l i:
-    Γ s⊨ tv va : oTTMem l L U, i -∗
-    Γ s⊨ oLater L, i <: oTSel (pv va) l, i.
-  Proof.
-    iIntros "#Hva !>" (ρ v) "#Hg #HvL".
-    iSpecialize ("Hva" with "Hg"). rewrite /= wp_value_inv' path_wp_pv.
-    iNext.
-    iDestruct "Hva" as (d Hl ψ) "#[Hlψ [#HLψ #HψU]]".
-    iExists ψ, d; repeat iSplit => //. by iApply "HLψ".
-  Qed.
-
-  Lemma Sel_Sub Γ L U va l i:
-    Γ s⊨ tv va : oTTMem l L U, i -∗
-    Γ s⊨ oTSel (pv va) l, i <: oLater U, i.
-  Proof.
-    iIntros "#Hva !>" (ρ v) "#Hg #Hψ".
-    iSpecialize ("Hva" with "Hg"); rewrite /= wp_value_inv' path_wp_pv.
-    iNext.
-    iDestruct "Hva" as (d Hl ψ) "#[Hlψ [#HLψ #HψU]]".
-    iDestruct "Hψ" as (ψ1 d1 Hva) "[Hγ #Hψ1v]".
-    objLookupDet. iDestruct (dm_to_type_agree d _ _ _ vnil v with "Hlψ Hγ") as "#Hag".
-    iApply "HψU" => //. iNext. by iRewrite "Hag".
-  Qed.
-
-(*
-  (* Alternative (and failed) definition. *)
-  Program Definition sem_sel p (l : label) :=
-    olty0 (λ ρ v, path_wp p.|[ρ]
-      (λ vp, ∃ ψ d, ⌜vp @ l ↘ d⌝ ∧ d ↗ ψ ∧ □ ψ v)%I).
-
-  Lemma Sub_Sel2 Γ L U va l i:
-    Γ s⊨ tv va : oTTMem l L U, i -∗
-    Γ s⊨ oLater L, i <: oLater (sem_sel (pv va) l), i.
-  Proof.
-    iIntros "/= #[% #Hva] !>" (ρ v Hclv) "#Hg #[_ HvL]". move: H => Hclva. iFrame (Hclv).
-    iSpecialize ("Hva" with "Hg"); rewrite wp_value_inv'.
-    iNext.
-
-    iDestruct "Hva" as (Hclvas' d Hl ψ) "#[Hlψ [#HLψ ?]]".
-    iSpecialize ("HLψ" $! _ Hclv with "HvL").
-    rewrite -later_intuitionistically.
-    iExists ψ, d; by repeat iSplit.
-  Qed.
-
-  Lemma Sel_Sub2_Failed Γ L U va l i:
-    Γ s⊨ tv va : oTTMem l L U, i -∗
-    Γ s⊨ oLater ((sem_sel (pv va) l)), i <: oLater U, i.
-  Proof.
-    iIntros "/= #[% #Hva] !>" (ρ v Hclv) "#Hg #[$ #[_ Hψ]]".
-    iSpecialize ("Hva" with "Hg"); rewrite wp_value_inv'.
-    iNext.
-    iDestruct "Hva" as (Hclvas d Hl ψ) "#[Hlψ [_ #HψU]]".
-    iApply "HψU" => //.
-    rewrite -later_intuitionistically.
-    iDestruct "Hψ" as (ψ1 d1) "[>% [Hγ #Hψ1v]]".
-    (* iSpecialize ("HLψ" $! v Hclv); iSpecialize ("HψU" $! v Hclv). *)
-    (* rewrite /sem_sel /olty_car. *)
-    objLookupDet; subst. iNext. iDestruct (dm_to_type_agree d _ _ v with "Hlψ Hγ") as "#Hag".
-    repeat iModIntro. Fail by iRewrite "Hag".
-  Abort. *)
-End SemTypes.
-
-(*
-  Even if semantic types use infinite substitutions, we can still reuse the
-  current stamping theory, based on finite substitutions.
-*)
-Section Sec.
-  Context `{HdotG: dlangG Σ} {i : nat}.
-  Implicit Types (φ : hoEnvD Σ i) (τ : olty Σ i).
-
-  Definition leadsto_envD_equiv s σ (φ : hoEnvD Σ i) : iProp Σ :=
-    (∃ (φ' : hoEnvD Σ i),
-      ⌜φ ≡ (λ args ρ, φ' args (∞ σ.|[ρ]))⌝ ∧ s ↝n[ i ] φ')%I.
-  Arguments leadsto_envD_equiv /.
-End Sec.
-
-Notation "s ↝[  σ  ] φ" := (leadsto_envD_equiv s σ φ) (at level 20).
-
-Section Sec2.
-  Context `{HdotG: dlangG Σ}.
-
-  Section with_unary_lr.
   Import stamp_transfer unary_lr.
 
   Lemma extraction_to_leadsto_envD_equiv T g s σ n: T ~[ n ] (g, (s, σ)) →
@@ -272,30 +113,7 @@ Section Sec2.
     - iIntros "!%" (args ρ v). exact: interp_subst_commute.
     - iApply (wellMappedφ_apply with "Hm"). by rewrite lookup_fmap Hl.
   Qed.
-  End with_unary_lr.
-
-  Lemma D_Typ_Abs Γ T L U s σ l :
-    Γ s⊨ T, 1 <: U, 1 -∗
-    Γ s⊨ L, 1 <: T, 1 -∗
-    s ↝[ σ ] T -∗
-    Γ s⊨ { l := dtysem σ s } : oDTMem l L U.
-  Proof.
-    iIntros "#HTU #HLT #Hs /="; iSplit => //.
-    iIntros "!>" (ρ) "#Hg /=".
-    iDestruct "Hs" as (φ Hγφ) "Hγ".
-    rewrite /dlty_car /=.
-    iExists (hoEnvD_inst (σ.|[ρ]) φ); iSplit.
-    by iApply dm_to_type_intro.
-    iModIntro; repeat iSplit; iIntros (v) "#HL"; rewrite later_intuitionistically.
-    - iIntros "!>". iApply Hγφ. by iApply "HLT".
-    - iApply "HTU" => //. by iApply Hγφ.
-  Qed.
-
-  Lemma D_Typ Γ (τ : olty Σ 0) s σ l:
-    s ↝[ σ ] τ -∗
-    Γ s⊨ { l := dtysem σ s } : oDTMem l τ τ.
-  Proof. iIntros "#Hs"; iApply D_Typ_Abs; by [| iIntros "!> **"]. Qed.
-End Sec2.
+End with_unary_lr.
 
 Section with_lty.
   Context `{dlangG Σ}.
@@ -406,4 +224,4 @@ Section with_lty.
     by eapply alias_paths_sameres, alias_paths_pself.
   Qed.
   End with_lty.
-End SemTypes.
+End SemTypes2.
