theories/Dot/misc_unused/dot_lty.v
@@ -1,0 +1,183 @@
+From iris.proofmode Require Import tactics.
+From D Require Import iris_prelude lty.
+From D.Dot Require Import syn syn.path_repl dlang_inst path_wp lr_syn_aux.
+From D.pure_program_logic Require Import lifting.
+
+Notation "'λI' x .. y , t" := (fun x => .. (fun y => t%I) ..)
+  (at level 200, x binder, y binder, right associativity, only parsing,
+  format "'[  ' '[  ' 'λI'  x  ..  y ']' ,  '/' t ']'") : function_scope.
+
+Implicit Types (Σ : gFunctors).
+Implicit Types
+         (v w : vl) (e : tm) (d : dm) (ds : dms) (p : path)
+         (vs : vls) (ρ : var → vl).
+
+Module SemTypes.
+
+Include LtyJudgements VlSorts dlang_inst.
+
+Record dlty Σ := Dlty {
+  dlty_label : label;
+  dlty_car : env -d> dm -d> iPropO Σ;
+  dlty_persistent ρ d :> Persistent (dlty_car ρ d);
+}.
+Global Arguments Dlty {_} _%I _ {_}.
+Global Arguments dlty_car {_} !_ _ _ /.
+Global Arguments dlty_label {_} _ /.
+Global Existing Instance dlty_persistent.
+
+
+(* Definition sdtp `{!dlangG Σ} Γ l (φ : dlty Σ) d : iProp Σ :=
+  □∀ ρ, ⌜path_includes (pv (ids 0)) ρ [(l, d)] ⌝ → s⟦Γ⟧* ρ → lift_dlty φ l ρ d.|[ρ]. *)
+
+Definition sdtp `{!dlangG Σ} Γ l (φ : dlty Σ) d : iProp Σ :=
+  (⌜ l = dlty_label φ ⌝ ∧
+    □∀ ρ, s⟦Γ⟧* ρ → dlty_car φ ρ d.|[ρ])%I.
+Global Arguments sdtp /.
+Notation "Γ s⊨ { l := d  } : T" := (sdtp Γ l T d) (at level 64, d, l, T at next level).
+
+Definition sptp `{!dlangG Σ} Γ (τ : olty Σ 0) p i: iProp Σ :=
+  □∀ ρ, s⟦Γ⟧* ρ -∗
+    ▷^i path_wp (p.|[ρ]) (λ v, oClose τ ρ v).
+
+Notation "Γ s⊨p p : τ , i" := (sptp Γ τ p i) (at level 74, p, τ, i at next level).
+
+(*
+  Even if semantic types use infinite substitutions, we can still reuse the
+  current stamping theory, based on finite substitutions.
+*)
+Section Sec.
+  Context `{HdotG: dlangG Σ} {i : nat}.
+  Implicit Types (φ : hoEnvD Σ i) (τ : olty Σ i).
+
+  Definition leadsto_envD_equiv s σ (φ : hoEnvD Σ i) : iProp Σ :=
+    (∃ (φ' : hoEnvD Σ i),
+      ⌜φ ≡ (λ args ρ, φ' args (∞ σ.|[ρ]))⌝ ∧ s ↝n[ i ] φ')%I.
+  Arguments leadsto_envD_equiv /.
+
+  Definition dm_to_type d i (ψ : hoD Σ i) : iProp Σ :=
+    (∃ s σ, ⌜ d = dtysem σ s ⌝ ∧ s ↗n[ σ , i ] ψ)%I.
+End Sec.
+
+Notation "s ↝[  σ  ] φ" := (leadsto_envD_equiv s σ φ) (at level 20).
+Notation "d ↗n[ i  ] ψ" := (dm_to_type d i ψ) (at level 20).
+
+Section dm_to_type.
+  Context `{HdotG: dlangG Σ}.
+  Global Instance dm_to_type_persistent d i ψ: Persistent (d ↗n[ i ] ψ) := _.
+
+  Lemma dm_to_type_agree d i ψ1 ψ2 args v : d ↗n[ i ] ψ1 -∗ d ↗n[ i ] ψ2 -∗ ▷ (ψ1 args v ≡ ψ2 args v).
+  Proof.
+    iDestruct 1 as (s σ ?) "#Hs1".
+    iDestruct 1 as (s' σ' ?) "#Hs2".
+    simplify_eq. by iApply (stamp_σ_to_type_agree args with "Hs1 Hs2").
+  Qed.
+
+  Lemma dm_to_type_intro d i s σ φ :
+    d = dtysem σ s → s ↝n[ i ] φ -∗ d ↗n[ i ] hoEnvD_inst σ φ.
+  Proof.
+    iIntros. iExists s, σ. iFrame "%".
+    by iApply stamp_σ_to_type_intro.
+  Qed.
+
+  Definition dm_to_type_eq d i ψ : dm_to_type d i ψ =
+    (∃ s σ, ⌜ d = dtysem σ s ⌝ ∧ s ↗n[ σ , i ] ψ)%I := eq_refl.
+
+  Global Opaque dm_to_type.
+End dm_to_type.
+
+
+Section SemTypes.
+  Context `{HdotG: dlangG Σ}.
+
+  Implicit Types (τ : olty Σ 0).
+   (* (ψ : vl -d> iPropO Σ) (φ : envD Σ)  *)
+
+  Program Definition lift_dinterp_vl (T : dlty Σ): olty Σ 0 :=
+    olty0 (λ ρ v, (∃ d, ⌜v @ dlty_label T ↘ d⌝ ∧ dlty_car T ρ d)%I).
+
+  (* Rewrite using (higher) semantic kinds! *)
+  Definition oDTMem l τ1 τ2 : dlty Σ := Dlty l
+    (λ ρ d,
+    ∃ ψ, (d ↗n[ 0 ] ψ) ∧
+       □ ((∀ v, ▷ τ1 vnil ρ v → ▷ □ ψ vnil v) ∧
+          (∀ v, ▷ □ ψ vnil v → ▷ τ2 vnil ρ v)))%I.
+
+  Definition oTTMem l τ1 τ2 :=
+    lift_dinterp_vl (oDTMem l τ1 τ2).
+
+  Definition oDVMem l τ : dlty Σ := Dlty l
+    (λ ρ d, ∃ pmem, ⌜d = dpt pmem⌝ ∧ path_wp pmem (oClose τ ρ))%I.
+
+  Definition oTVMem l τ :=
+    lift_dinterp_vl (oDVMem l τ).
+(*
+  Program Definition oInterp T := Olty ⟦ T ⟧ _.
+  Next Obligation. rewrite /vclosed=>*. by rewrite interp_vclosed. Qed. *)
+
+  Definition oTSel p (l : label) :=
+    olty0 (λ ρ v, path_wp p.|[ρ]
+      (λ vp, ∃ ψ d, ⌜vp @ l ↘ d⌝ ∧ d ↗n[ 0 ] ψ ∧ ▷ □ ψ vnil v))%I.
+
+  Lemma oTSel_pv w (l : label) args ρ v :
+    oTSel (pv w) l args ρ v ≡
+      (∃ ψ d, ⌜w.[ρ] @ l ↘ d⌝ ∧ d ↗n[ 0 ] ψ ∧ ▷ □ ψ vnil v)%I.
+  Proof. by rewrite /= path_wp_pv. Qed.
+
+  Definition oPSing p : olty Σ 0 :=
+    olty0 (λI ρ v, ⌜alias_paths p.|[ρ] (pv v)⌝).
+End SemTypes.
+
+Section SampleTypingLemmas.
+  Context `{HdotG: dlangG Σ}.
+
+  Implicit Types (τ L T U : olty Σ 0).
+
+  Lemma Sub_Sel Γ L U va l i:
+    Γ s⊨ tv va : oTTMem l L U, i -∗
+    Γ s⊨ oLater L, i <: oTSel (pv va) l, i.
+  Proof.
+    iIntros "#Hva !>" (ρ v) "#Hg #HvL".
+    iSpecialize ("Hva" with "Hg"). rewrite /= wp_value_inv' path_wp_pv.
+    iNext.
+    iDestruct "Hva" as (d Hl ψ) "#[Hlψ [#HLψ #HψU]]".
+    iExists ψ, d; repeat iSplit => //. by iApply "HLψ".
+  Qed.
+
+  Lemma Sel_Sub Γ L U va l i:
+    Γ s⊨ tv va : oTTMem l L U, i -∗
+    Γ s⊨ oTSel (pv va) l, i <: oLater U, i.
+  Proof.
+    iIntros "#Hva !>" (ρ v) "#Hg #Hψ".
+    iSpecialize ("Hva" with "Hg"); rewrite /= wp_value_inv' path_wp_pv.
+    iNext.
+    iDestruct "Hva" as (d Hl ψ) "#[Hlψ [#HLψ #HψU]]".
+    iDestruct "Hψ" as (ψ1 d1 Hva) "[Hγ #Hψ1v]".
+    objLookupDet. iDestruct (dm_to_type_agree d _ _ _ vnil v with "Hlψ Hγ") as "#Hag".
+    iApply "HψU" => //. iNext. by iRewrite "Hag".
+  Qed.
+
+  Lemma D_Typ_Abs Γ T L U s σ l :
+    Γ s⊨ T, 1 <: U, 1 -∗
+    Γ s⊨ L, 1 <: T, 1 -∗
+    s ↝[ σ ] T -∗
+    Γ s⊨ { l := dtysem σ s } : oDTMem l L U.
+  Proof.
+    iIntros "#HTU #HLT #Hs /="; iSplit => //.
+    iIntros "!>" (ρ) "#Hg /=".
+    iDestruct "Hs" as (φ Hγφ) "Hγ".
+    rewrite /dlty_car /=.
+    iExists (hoEnvD_inst (σ.|[ρ]) φ); iSplit.
+    by iApply dm_to_type_intro.
+    iModIntro; repeat iSplit; iIntros (v) "#HL"; rewrite later_intuitionistically.
+    - iIntros "!>". iApply Hγφ. by iApply "HLT".
+    - iApply "HTU" => //. by iApply Hγφ.
+  Qed.
+
+  Lemma D_Typ Γ (τ : olty Σ 0) s σ l:
+    s ↝[ σ ] τ -∗
+    Γ s⊨ { l := dtysem σ s } : oDTMem l τ τ.
+  Proof. iIntros "#Hs"; iApply D_Typ_Abs; by [| iIntros "!> **"]. Qed.
+End SampleTypingLemmas.
+
+End SemTypes.
